theories/check1.v
@@ -2465,67 +2465,6 @@ Section more_precise.
   Print Assumptions more_precise_tc_tree_aux.
 End more_precise.
 
-
-Definition typ_func (A: typecheck (_ * sigV)%type) := match A with ty_ok (Func, _) => true | _ => false end.
-
-Lemma all_det_nfa_big_and {sP sV l r} p: 
-  valid_sig sV ->
-  typ_func (check_atoms sP sV l r)-> 
-    typ_func (tc_tree_aux sP sV (big_and p l) r).
-Proof.
-  elim: l sV r => //=.
-  move=> A As IH sV r V.
-  case X: check_atom => /=[[dA sVA]|]//=.
-  case YY : A X => //=[|c].
-    move=> [??]; subst => //=.
-    move=> {}/IH H.
-    have {H}:= H V.
-    case dt: tc_tree_aux V => //=[[[b|]]]//= V _.
-    rewrite merge_refl//=.
-    apply: tc_tree_aux_valid_sig V dt.
-  rewrite/check_callable.
-  case X: check_tm => //[[[d b]|]]//=; last first.
-    case G: get_callable_hd_sig => [S|]//=; last first.
-      move=> [??]; subst => /=; rewrite maxD_comm/=.
-      move=> /IH/= -/(_ V); case dtA: tc_tree_aux => //=[[[b|]]]//=.
-      rewrite merge_refl//=.
-      apply: tc_tree_aux_valid_sig V dtA.
-    case Ass: assume_call => //=[V'][??]; subst => /=.
-    have H1 := assume_call_valid_sig V Ass.
-    move=> /IH -/(_ H1).
-    rewrite maxD_comm/=.
-    case dt: tc_tree_aux => //=[[[]S1]]//= _.
-    rewrite merge_refl//.
-    by apply: tc_tree_aux_valid_sig dt.
-  case: d X => //-[]//=d.
-  case Y: get_callable_hd_sig => //[s|].
-    case: b => //=.
-      case X: assume_call => //=[ts] H [??]; subst.
-      have H1 := assume_call_valid_sig V X.
-      move=> /IH -/(_ H1).
-      rewrite maxD_comm maxD_assoc maxD_refl.
-      case dt: tc_tree_aux => //=[[[]S]]//= _.
-      rewrite merge_refl//=.
-      apply: tc_tree_aux_valid_sig H1 dt.
-    move=> H [??]; subst => /IH -/(_ V).
-    rewrite maxD_comm/=.
-    case dt: tc_tree_aux => //[[[]b]]//=.
-    rewrite merge_refl//=.
-    apply: tc_tree_aux_valid_sig V dt.
-  case: b => //=.
-    move=> H [??]; subst.
-    move=> /IH-/(_ V).
-    rewrite maxD_comm/=.
-    case dt: tc_tree_aux => //[[[]S]]//= _.
-    rewrite merge_refl//=.
-    apply: tc_tree_aux_valid_sig V dt.
-  move=> H [??]; subst => /IH -/(_ V).
-  rewrite maxD_comm/=.
-  case dt: tc_tree_aux => //[[[]S]]//= _.
-  rewrite merge_refl//=.
-  apply: tc_tree_aux_valid_sig V dt.
-Qed.
-
 Lemma deterf_empty c: 
   deref empty c = c.
 Proof. elim: c => //= t IH tm H; rewrite IH//. Qed.
